## [Section 1.2 - Procedures and the Processes They Generate](https://mitpress.mit.edu/sicp/full-text/book/book-Z-H-11.html#%_sec_1.2)

## Exercises
**Exercise 1.9** Each of the following two procedures defines a method for adding two positive integers in terms of the procedures inc, which increments its argument by 1, and dec, which decrements its argument by 1.
```scheme
(define (+ a b)
  (if (= a 0)
      b
      (inc (+ (dec a) b))))

(define (+ a b)
  (if (= a 0)
      b
      (+ (dec a) (inc b))))
```
Using the substitution model, illustrate the process generated by each procedure in evaluating (+ 4 5). Are these processes iterative or recursive?

**Exercise 1.10** The following procedure computes a mathematical function called Ackermann's function.
```scheme
(define (A x y)
  (cond ((= y 0) 0)
        ((= x 0) (* 2 y))
        ((= y 1) 2)
        (else (A (- x 1)
                 (A x (- y 1))))))
```
What are the values of the following expressions?
```scheme
(A 1 10)
(A 2 4)
(A 3 3)
```
Consider the following procedures, where A is the procedure defined above:
```scheme
(define (f n) (A 0 n))
(define (g n) (A 1 n))
(define (h n) (A 2 n))
(define (k n) (* 5 n n))
```
Give concise mathematical definitions for the functions computed by the procedures f, g, and h for positive integer values of n. For example, (k n) computes 5n^2.

```scheme
(A 1 10)
; 2^10 because the final argument, (A x (- y 1))
;       will evaluate 9 times before y = 1 and the
;       function stops at 2
(A 2 4)
; 2^16 because the function first evaluates to (A 1 (A 2 3))
;       = (A 1 (A 1 (A 2 2)))
;       = (A 1 (A 1 (A 1 (A 2 1))))
;       = (A 1 (A 1 (A 1 2)))
;       = (A 1 (A 1 (A 0 (A 1 1))))
;       = (A 1 (A 1 (A 0 2)))
;       = (A 1 (A 1 (2 * 2)))
;       = (A 1 (A 1 4))
;       = (A 1 (A 0 (A 1 3)))
;       = (A 1 (A 0 (A 0 (A 1 2))))
;       = (A 1 (A 0 (A 0 (A 1 2))))
;       = (A 1 (A 0 (A 0 (A 0 (A 1 1)))))
;       = (A 1 (A 0 (A 0 (A 0 2))))
;       = (A 1 (A 0 (A 0 (2 * 2))))
;       = (A 1 (A 0 (A 0 4)))
;       = (A 1 (A 0 (2 * 4)))
;       = (A 1 (A 0 8))
;       = (A 1 (2 * 8))
;       = (A 1 16)
;       which as we saw above will evaluate to 2^16
(A 3 3)
; 2^16 because the function first evaluates to (A 2 (A 3 2))
;       = (A 2 (A 2 (A 3 1)))
;       = (A 2 (A 2 2))
;       = (A 2 (A 1 (A 2 1)))
;       = (A 2 (A 1 2))
;       = (A 2 (A 0 (A 1 1)))
;       = (A 2 (A 0 2))
;       = (A 2 (2 * 2))
;       = (A 2 4)
;       which as we saw above will evaluate to 2^16

(define (f n) (A 0 n))
; f(n) = 2*n
(define (g n) (A 1 n))
; g(n) = 2^n
(define (h n) (A 2 n))
; h(n) = 2^(n^2)
```

**Exercise 1.11** A function f is defined by the rule that f(n) = n if n < 3 and f(n) = f(n-1) + f(n-2) + f(n-3) if n >= 3.  
Write a procedure that computes f by means of a recursive process. Write a procedure that computes f by means of an iterative process.
```scheme
; Recursive solution
(define (f n)
  (cond ((< n 3) n)
	     (else (+ (+ (f (- n 1)) (* 2 (f (- n 2)))) (* 3 (f (- n 3)))))))
; Iterative solution
; a <- a + 2*b + 3*c
; b <- a
; c <- b
(define (f n)
  (f-iter 2 1 0 n))
(define (f-iter a b c count)
  (if (= count 0)
      c
      (f-iter (+ a (* b 2) (* c 3)) a b (- count 1))))
```

**Exercise 1.12** The following pattern of numbers is called Pascal's triangle.  
&nbsp;&nbsp;&nbsp;&nbsp;&nbsp;&nbsp;&nbsp;&nbsp;1  
&nbsp;&nbsp;&nbsp;&nbsp;&nbsp;&nbsp;&nbsp;1&nbsp;1  
&nbsp;&nbsp;&nbsp;&nbsp;&nbsp;&nbsp;1&nbsp;2&nbsp;1  
&nbsp;&nbsp;&nbsp;&nbsp;&nbsp;1&nbsp;3&nbsp;3&nbsp;1  
&nbsp;&nbsp;&nbsp;&nbsp;1&nbsp;4&nbsp;6&nbsp;4&nbsp;1  
The numbers at the edge of the triangle are all 1, and each number inside the triangle is the sum of the two numbers above it.35 Write a procedure that computes elements of Pascal's triangle by means of a recursive process.
```scheme
(define (pascal row col)
  (cond ((= row 1) 1)
	    ((= row col) 1)
	    ((= col 1) 1)
        (else (+ (pascal (- row 1) (- col 1))
		         (pascal (- row 1) col)))))
(pascal 1 1)
;Value: 1
(pascal 2 1)
;Value: 1
(pascal 2 2)
;Value: 1
(pascal 3 1)
;Value: 1
(pascal 3 2)
;Value: 2
(pascal 3 3)
;Value: 1
(pascal 4 2)
;Value: 3
(pascal 4 3)
;Value: 3
(pascal 5 3)
;Value: 6
```

**Exercise 1.13** Prove that Fib(n) is the closest integer to (phi^n)/5, where phi = (1 + sqrt(5))/2. Hint: Let psi = (1 - sqrt(5))/2. Use induction and the definition of the Fibonacci numbers (see section 1.2.2) to prove that Fib(n) = (n - n)/5.

| Base case: | show for n = 0 and n = 1 |
| ------------- |:-------------|
| n=0 | Fib(0) = (phi^0 - rho^0)/sqrt(5) |
| | 0 = (0 - 0)/sqrt(5) |
| | 0 = 0 |
| n=1 | Fib(1) = (phi^1 - rho^1)/sqrt(5) |
| | 1 = ((1 + sqrt(5))/2 - (1 - sqrt(5))/2)/sqrt(5) |
| | 1 = ((2*(sqrt(5)))/2) / sqrt(5) |
| | 1 = (sqrt(5)) / sqrt(5) |
| | 1 = 1 |  

| Induction case: | take k >= 1 as given and assume relation is true for all n >= 0 |
| ------------- |:-------------|
| | Fib(k + 1) = Fib(k) + Fib(k - 1) |
| by induction hypothesis | Fib(k + 1) = ((phi^(k) - rho^(k))/sqrt(5)) + ((phi^(k - 1) - rho^(k - 1))/sqrt(5)) |
| | Fib(k + 1) = ((phi)^(k) + (phi)^(k - 1))/sqrt(5) - ((rho)^(k) + (rho)^(k - 1))/sqrt(5) |
| since phi^2 = phi + 1 and rho^2 = rho + 1 | Fib(k + 1) = (((phi)^(k - 1)(phi + 1)) - ((rho)^(k - 1)(rho + 1)))/sqrt(5) |
| | Fib(k + 1) = (((phi)^(k - 1)(phi^2)) - ((rho)^(k - 1)(rho^2)))/sqrt(5) |
| | Fib(k + 1) = ((phi)^(k + 1) - (rho)^(k + 1))/sqrt(5) |

**Exercise 1.14** Draw the tree illustrating the process generated by the count-change procedure of section 1.2.2 in making change for 11 cents. What are the orders of growth of the space and number of steps used by this process as the amount to be changed increases?
